some stylistic changes

code/experimental/P256/ecdsap256-c/Hacl_Impl_ECDSA_P256SHA256_Signature.c
@@ -9,9 +9,9 @@
 
 void
 Hacl_Impl_ECDSA_P256SHA256_Signature_ecdsa_signature_step12(
+  uint64_t *hashAsFelem,
   uint32_t mLen,
-  uint8_t *m,
-  uint64_t *hashAsFelem
+  uint8_t *m
 )
 {
   uint8_t mHash[32U] = { 0U };
@@ -23,9 +23,9 @@ Hacl_Impl_ECDSA_P256SHA256_Signature_ecdsa_signature_step12(
 
 bool
 Hacl_Impl_ECDSA_P256SHA256_Signature_ecdsa_signature_step45(
+  uint64_t *x,
   uint8_t *k,
-  uint64_t *tempBuffer,
-  uint64_t *x
+  uint64_t *tempBuffer
 )
 {
   uint64_t result[12U] = { 0U };
@@ -38,11 +38,11 @@ Hacl_Impl_ECDSA_P256SHA256_Signature_ecdsa_signature_step45(
 
 void
 Hacl_Impl_ECDSA_P256SHA256_Signature_ecdsa_signature_step6(
+  uint64_t *result,
   uint64_t *kFelem,
   uint64_t *z,
   uint64_t *r,
-  uint64_t *da,
-  uint64_t *result
+  uint64_t *da
 )
 {
   uint64_t rda[4U] = { 0U };
@@ -58,27 +58,13 @@ Hacl_Impl_ECDSA_P256SHA256_Signature_ecdsa_signature_step6(
     result);
 }
 
-void Hacl_Impl_ECDSA_P256SHA256_Signature_toUint64(uint8_t *i, uint64_t *o)
-{
-  uint32_t i0;
-  for (i0 = (uint32_t)0U; i0 < (uint32_t)4U; i0 = i0 + (uint32_t)1U)
-  {
-    uint64_t *os = o;
-    uint8_t *bj = i + i0 * (uint32_t)8U;
-    uint64_t u = load64_le(bj);
-    uint64_t r = u;
-    uint64_t x = r;
-    os[i0] = x;
-  }
-}
-
 bool
 Hacl_Impl_ECDSA_P256SHA256_Signature_ecdsa_signature_core_nist_compliant(
+  uint64_t *r,
+  uint64_t *s1,
   uint8_t *m,
   uint64_t *privKeyAsFelem,
-  uint8_t *k,
-  uint64_t *r,
-  uint64_t *s1
+  uint8_t *k
 )
 {
   uint64_t hashAsFelem[4U] = { 0U };
@@ -87,16 +73,16 @@ Hacl_Impl_ECDSA_P256SHA256_Signature_ecdsa_signature_core_nist_compliant(
   uint64_t hashAsFelem1[4U] = { 0U };
   bool step5Flag;
   bool ite;
-  Hacl_Impl_ECDSA_P256SHA256_Signature_toUint64(m, hashAsFelem1);
-  Hacl_Impl_ECDSA_P256SHA256_Signature_toUint64(k, kAsFelem);
-  step5Flag = Hacl_Impl_ECDSA_P256SHA256_Signature_ecdsa_signature_step45(k, tempBuffer, r);
+  Hacl_Impl_ECDSA_P256SHA256_Common_toUint64(m, hashAsFelem1);
+  Hacl_Impl_ECDSA_P256SHA256_Common_toUint64(k, kAsFelem);
+  step5Flag = Hacl_Impl_ECDSA_P256SHA256_Signature_ecdsa_signature_step45(r, k, tempBuffer);
   if (!step5Flag)
   {
-    Hacl_Impl_ECDSA_P256SHA256_Signature_ecdsa_signature_step6(kAsFelem,
+    Hacl_Impl_ECDSA_P256SHA256_Signature_ecdsa_signature_step6(s1,
+      kAsFelem,
       hashAsFelem1,
       r,
-      privKeyAsFelem,
-      s1);
+      privKeyAsFelem);
     {
       bool step6Flag = Hacl_Impl_LowLevel_isZero_bool(s1);
       ite = !step6Flag;
@@ -111,10 +97,10 @@ Hacl_Impl_ECDSA_P256SHA256_Signature_ecdsa_signature_core_nist_compliant(
 
 bool
 Hacl_Impl_ECDSA_P256SHA256_Signature_ecdsa_signature_nist_compliant(
+  uint8_t *result,
   uint8_t *m,
   uint8_t *privKey,
-  uint8_t *k,
-  uint8_t *result
+  uint8_t *k
 )
 {
   uint64_t privKeyAsFelem[4U] = { 0U };
@@ -123,13 +109,13 @@ Hacl_Impl_ECDSA_P256SHA256_Signature_ecdsa_signature_nist_compliant(
   uint8_t *resultR = result;
   uint8_t *resultS = result + (uint32_t)32U;
   bool flag;
-  Hacl_Impl_ECDSA_P256SHA256_Signature_toUint64(privKey, privKeyAsFelem);
+  Hacl_Impl_ECDSA_P256SHA256_Common_toUint64(privKey, privKeyAsFelem);
   flag =
-    Hacl_Impl_ECDSA_P256SHA256_Signature_ecdsa_signature_core_nist_compliant(m,
+    Hacl_Impl_ECDSA_P256SHA256_Signature_ecdsa_signature_core_nist_compliant(r,
+      s1,
+      m,
       privKeyAsFelem,
-      k,
-      r,
-      s1);
+      k);
   Hacl_Impl_ECDSA_P256SHA256_Common_toUint8(r, resultR);
   Hacl_Impl_ECDSA_P256SHA256_Common_toUint8(s1, resultS);
   return flag;
@@ -150,16 +136,16 @@ Hacl_Impl_ECDSA_P256SHA256_Signature_ecdsa_signature_core(
   uint64_t kAsFelem[4U] = { 0U };
   bool step5Flag;
   bool ite;
-  Hacl_Impl_ECDSA_P256SHA256_Signature_toUint64(k, kAsFelem);
-  Hacl_Impl_ECDSA_P256SHA256_Signature_ecdsa_signature_step12(mLen, m, hashAsFelem);
-  step5Flag = Hacl_Impl_ECDSA_P256SHA256_Signature_ecdsa_signature_step45(k, tempBuffer, r);
+  Hacl_Impl_ECDSA_P256SHA256_Common_toUint64(k, kAsFelem);
+  Hacl_Impl_ECDSA_P256SHA256_Signature_ecdsa_signature_step12(hashAsFelem, mLen, m);
+  step5Flag = Hacl_Impl_ECDSA_P256SHA256_Signature_ecdsa_signature_step45(r, k, tempBuffer);
   if (!step5Flag)
   {
-    Hacl_Impl_ECDSA_P256SHA256_Signature_ecdsa_signature_step6(kAsFelem,
+    Hacl_Impl_ECDSA_P256SHA256_Signature_ecdsa_signature_step6(s1,
+      kAsFelem,
       hashAsFelem,
       r,
-      privKeyAsFelem,
-      s1);
+      privKeyAsFelem);
     {
       bool step6Flag = Hacl_Impl_LowLevel_isZero_bool(s1);
       ite = !step6Flag;
@@ -187,7 +173,7 @@ Hacl_Impl_ECDSA_P256SHA256_Signature_ecdsa_signature(
   uint8_t *resultR = result;
   uint8_t *resultS = result + (uint32_t)32U;
   bool flag;
-  Hacl_Impl_ECDSA_P256SHA256_Signature_toUint64(privKey, privKeyAsFelem);
+  Hacl_Impl_ECDSA_P256SHA256_Common_toUint64(privKey, privKeyAsFelem);
   flag =
     Hacl_Impl_ECDSA_P256SHA256_Signature_ecdsa_signature_core(mLen,
       m,
