code/experimental/P256/Hacl.Impl.ECDSA.P256SHA256.Signature.fst
@@ -6,6 +6,7 @@ module ST = FStar.HyperStack.ST
 
 open Lib.IntTypes
 open Lib.Buffer
+open Lib.ByteSequence
 
 open Hacl.Hash.SHA2
 open Hacl.Spec.P256.Definitions
@@ -30,46 +31,9 @@ open FStar.Mul
 
 #set-options "--z3rlimit 100"
 
-val lemma_core_0: a: lbuffer uint64 (size 4) -> h: mem -> 
-  Lemma (Lib.ByteSequence.nat_from_intseq_le (as_seq h a) == as_nat h a)
-
-let lemma_core_0 a h = 
-  let open Lib.ByteSequence in 
-  
-    let k = as_seq h a in 
-    let z = nat_from_intseq_le k in 
-    
-    nat_from_intseq_le_slice_lemma k 1;
-    nat_from_intseq_le_lemma0 (Seq.slice k 0 1);
-
-    let k1 = Seq.slice k 1 4 in 
-      nat_from_intseq_le_slice_lemma #_ #_ #3 k1 1;
-      nat_from_intseq_le_lemma0 (Seq.slice k1 0 1);
-      
-    let k2 = Seq.slice k1 1 3 in 
-      nat_from_intseq_le_slice_lemma #_ #_ #2 k2 1;
-      nat_from_intseq_le_lemma0 (Seq.slice k2 0 1);
-      nat_from_intseq_le_lemma0 (Seq.slice k2 1 2)
-
-
-val lemma_core_1: a: lbuffer uint64 (size 4) -> h: mem -> 
-  Lemma (Lib.ByteSequence.nat_from_bytes_le (Lib.ByteSequence.uints_to_bytes_le (as_seq h a)) == as_nat h a)
-
-let lemma_core_1 a h= 
-  let open Lib.ByteSequence in 
-  let k = as_seq h a in 
-  let z = Lib.ByteSequence.uints_to_bytes_le (as_seq h a) in 
-  let maint = Lib.ByteSequence.nat_from_bytes_le (Lib.ByteSequence.uints_to_bytes_le (as_seq h a)) in 
-  lemma_core_0 a h;
-  lemma_nat_from_to_intseq_le_preserves_value #U64 #SEC 4 (as_seq h a);
-  let n = nat_from_intseq_le k in 
-  uints_to_bytes_le_nat_lemma #U64 #SEC 4 n;
-  lemma_nat_to_from_bytes_le_preserves_value #SEC (uints_to_bytes_le #U64 #SEC #4 (as_seq h a)) 32 (as_nat h a)
-
-
-val ecdsa_signature_step12: mLen: size_t -> m: lbuffer uint8 mLen {uint_v mLen < pow2 61} -> hashAsFelem: felem -> 
+val ecdsa_signature_step12: hashAsFelem: felem -> mLen: size_t -> m: lbuffer uint8 mLen {uint_v mLen < pow2 61} -> 
   Stack unit 
-    (requires fun h -> live h m /\ live h hashAsFelem)
+    (requires fun h -> live h hashAsFelem /\ live h m)
     (ensures fun h0 _ h1 -> modifies (loc hashAsFelem) h0 h1 /\
       (
 	let hashM = Spec.Hash.hash Spec.Hash.Definitions.SHA2_256 (as_seq h0 m) in 
@@ -78,24 +42,22 @@ val ecdsa_signature_step12: mLen: size_t -> m: lbuffer uint8 mLen {uint_v mLen <
       ) 
   ) 
 
-let ecdsa_signature_step12 mLen m hashAsFelem  = 
+let ecdsa_signature_step12 hashAsFelem mLen m  = 
   push_frame(); 
     let mHash = create (size 32) (u8 0) in  
       let h0 = ST.get() in 
     hash_256 m mLen mHash;
     toUint64ChangeEndian mHash hashAsFelem;
-      let h2 = ST.get() in 
-      lemma_core_0 hashAsFelem h2;
+      let h1 = ST.get() in 
+      lemma_core_0 hashAsFelem h1;
     reduction_prime_2prime_order hashAsFelem hashAsFelem;
   pop_frame()
 
 
-val ecdsa_signature_step45: k: lbuffer uint8 (size 32) -> 
-  tempBuffer: lbuffer uint64 (size 100) -> 
-  x: felem -> 
+val ecdsa_signature_step45: x: felem ->  k: lbuffer uint8 (size 32) -> tempBuffer: lbuffer uint64 (size 100) -> 
   Stack bool 
     (requires fun h -> 
-      live h k /\ live h x /\ live h tempBuffer /\ 
+      live h x /\ live h k /\ live h tempBuffer /\ 
       LowStar.Monotonic.Buffer.all_disjoint [loc tempBuffer; loc k; loc x]
     )
     (ensures fun h0 r h1 -> modifies (loc x |+| loc tempBuffer) h0 h1 /\
@@ -109,7 +71,7 @@ val ecdsa_signature_step45: k: lbuffer uint8 (size 32) ->
       )
     )
 
-let ecdsa_signature_step45 k tempBuffer x = 
+let ecdsa_signature_step45 x k tempBuffer= 
   push_frame();
       let result = create (size 12) (u64 0) in 
       let tempForNorm = sub tempBuffer (size 0) (size 88) in 
@@ -120,8 +82,8 @@ let ecdsa_signature_step45 k tempBuffer x =
     isZero_bool x
 
 
-val lemma_power_step6: kInv: nat  -> Lemma 
-  (Hacl.Spec.ECDSA.exponent_spec (fromDomain_ kInv)  == toDomain_ (pow kInv (prime_p256_order - 2)))
+val lemma_power_step6: kInv: nat -> Lemma 
+  (Hacl.Spec.ECDSA.exponent_spec (fromDomain_ kInv) == toDomain_ (pow kInv (prime_p256_order - 2)))
 
 let lemma_power_step6 kInv = 
   let a = Hacl.Spec.ECDSA.exponent_spec (fromDomain_ kInv) in 
@@ -131,7 +93,6 @@ let lemma_power_step6 kInv =
   power_distributivity_2 kInv (modp_inv2_prime (pow2 256) prime_p256_order % prime_p256_order) (prime_p256_order - 2);
   lemma_mod_mul_distr_r (pow kInv (prime_p256_order - 2)) (pow (modp_inv2_prime (pow2 256) prime_p256_order) (prime_p256_order - 2)) prime_p256_order;
 
-
   lemma_pow_mod_n_is_fpow prime_p256_order (pow2 256 % prime_p256_order) (prime_p256_order - 2);
   assert_norm(modp_inv2_prime (pow2 256) prime_p256_order = 43790243014242295660885426880012836369732278457577312309071968676491870960761); 
 
@@ -139,20 +100,21 @@ let lemma_power_step6 kInv =
   assert_norm(exp #prime_p256_order 43790243014242295660885426880012836369732278457577312309071968676491870960761 (prime_p256_order - 2) == pow2 256 % prime_p256_order);
 
   lemma_mod_mul_distr_r (pow kInv (prime_p256_order - 2)) (pow2 256) prime_p256_order;
-   lemmaToDomain (pow kInv (prime_p256_order - 2))
+  lemmaToDomain (pow kInv (prime_p256_order - 2))
 
 
 #reset-options "--z3rlimit 300"
 
-val ecdsa_signature_step6: kFelem: felem -> z: felem -> r: felem -> da: felem ->result: felem -> Stack unit
-  (requires fun h -> live h kFelem /\ live h z /\ live h r /\ live h da /\ 
-    as_nat h z < prime_p256_order /\ as_nat h r < prime_p256_order /\ as_nat h da < prime_p256_order /\ 
-    as_nat h kFelem < prime_p256_order /\ live h result)
+val ecdsa_signature_step6: result: felem -> kFelem: felem -> z: felem -> r: felem -> da: felem -> Stack unit
+  (requires fun h -> live h result /\ live h kFelem /\ live h z /\ live h r /\ live h da /\
+    as_nat h kFelem < prime_p256_order /\ as_nat h z < prime_p256_order /\ as_nat h r < prime_p256_order /\ 
+    as_nat h da < prime_p256_order
+  )
   (ensures fun h0 _ h1 -> modifies (loc result) h0 h1 /\
     as_nat h1 result = (as_nat h0 z + as_nat h0 r * as_nat h0 da) * pow (as_nat h0 kFelem) (prime_p256_order - 2) % prime_p256_order)
 
 
-let ecdsa_signature_step6 kFelem z r da result = 
+let ecdsa_signature_step6 result kFelem z r da = 
   let open FStar.Tactics in 
   let open FStar.Tactics.Canon in 
   push_frame();
@@ -197,32 +159,17 @@ let ecdsa_signature_step6 kFelem z r da result =
        lemma_mod_mul_distr_r br0 br1 prime_p256_order
 
 
-val toUint64: i: lbuffer uint8 (32ul) -> o: felem -> Stack unit
-  (requires fun h -> live h i /\ live h o /\ disjoint i o)
-  (ensures 
-    fun h0 _ h1 -> modifies (loc o) h0 h1 /\ 
-      as_seq h1 o == Lib.ByteSequence.uints_from_bytes_le (as_seq h0 i))
-
-let toUint64 i o = 
-    Lib.ByteBuffer.uints_from_bytes_le o i
-
-
-
-
-val ecdsa_signature_core_nist_compliant: m: lbuffer uint8 (size 32) -> 
-  privKeyAsFelem: felem -> 
+val ecdsa_signature_core_nist_compliant: r: felem -> s: felem -> m: lbuffer uint8 (size 32) -> privKeyAsFelem: felem -> 
   k: lbuffer uint8 (size 32) -> 
-  r: felem -> 
-  s: felem -> 
   Stack bool  
-  (requires fun h -> live h m /\ live h privKeyAsFelem /\ live h k /\ live h r /\ live h s /\ 
+  (requires fun h -> live h r /\ live h s /\ live h m /\ live h privKeyAsFelem /\ live h k /\ 
     disjoint privKeyAsFelem r /\ disjoint k r /\ disjoint r s /\
-    as_nat h privKeyAsFelem < prime_p256_order /\
     Lib.ByteSequence.nat_from_bytes_le (as_seq h m) < prime_p256_order /\
+    as_nat h privKeyAsFelem < prime_p256_order /\
     Lib.ByteSequence.nat_from_bytes_le (as_seq h k) < prime_p256_order
   )
   (ensures fun h0 flag h1 -> modifies (loc r |+| loc s) h0 h1 /\
-  (
+    (
       let basePoint = (0x6B17D1F2E12C4247F8BCE6E563A440F277037D812DEB33A0F4A13945D898C296, 0x4FE342E2FE1A7F9B8EE7EB4A7C0F9E162BCE33576B315ECECBB6406837BF51F5, 1) in
       let (rxN, ryN, rzN), _ = montgomery_ladder_spec (as_seq h0 k) ((0,0,0), basePoint) in 
       let (xN, _, _) = _norm (rxN, ryN, rzN) in 
@@ -237,48 +184,41 @@ val ecdsa_signature_core_nist_compliant: m: lbuffer uint8 (size 32) ->
 	)
       )
     )
-)
+  )
 
-
-
-let ecdsa_signature_core_nist_compliant m privKeyAsFelem k r s = 
+let ecdsa_signature_core_nist_compliant r s m privKeyAsFelem k = 
   push_frame();
-    let h0 = ST.get() in 
-      let open Lib.ByteSequence in 
-      let hashAsFelem = create (size 4) (u64 0) in     
-      let tempBuffer = create (size 100) (u64 0) in 
-      let kAsFelem = create (size 4) (u64 0) in 
-      let hashAsFelem = create (size 4) (u64 0) in 
-	toUint64 m hashAsFelem;
-	toUint64 k kAsFelem;
-	  
-	  let h1 = ST.get() in 
- 	    lemma_core_0 kAsFelem h1;
-	    uints_from_bytes_le_nat_lemma #U64 #_ #4 (as_seq h0 k);
+  let h0 = ST.get() in 
+    let hashAsFelem = create (size 4) (u64 0) in     
+    let tempBuffer = create (size 100) (u64 0) in 
+    let kAsFelem = create (size 4) (u64 0) in 
+    let hashAsFelem = create (size 4) (u64 0) in 
+    toUint64 m hashAsFelem;
+    toUint64 k kAsFelem;
+  let h1 = ST.get() in 
+      lemma_core_0 kAsFelem h1;
+      uints_from_bytes_le_nat_lemma #U64 #_ #4 (as_seq h0 k);
 
-	    lemma_core_0 hashAsFelem h1;
-	    uints_from_bytes_le_nat_lemma #U64 #_ #4 (as_seq h0 m);
-	    
-    let step5Flag = ecdsa_signature_step45 k tempBuffer r in 
-      if not step5Flag then begin
-	   ecdsa_signature_step6 kAsFelem hashAsFelem r privKeyAsFelem s;
-	   
+      lemma_core_0 hashAsFelem h1;
+      uints_from_bytes_le_nat_lemma #U64 #_ #4 (as_seq h0 m);
+  let step5Flag = ecdsa_signature_step45 r k tempBuffer in 
+    if not step5Flag then 
+      begin
+	ecdsa_signature_step6 s kAsFelem hashAsFelem r privKeyAsFelem;
 	pop_frame();
 	let step6Flag = isZero_bool s in 
 	not step6Flag
       end 
-      else 
-	begin
-	  pop_frame();
-	  false
+    else 
+      begin
+	pop_frame();
+	false
       end   
 
-open Lib.ByteSequence
-
-val ecdsa_signature_nist_compliant: m: lbuffer uint8 (size 32) -> 
+val ecdsa_signature_nist_compliant: result: lbuffer uint8 (size 64) -> m: lbuffer uint8 (size 32) -> 
   privKey: lbuffer uint8 (size 32) -> 
   k: lbuffer uint8 (size 32) -> 
-  result: lbuffer uint8 (size 64) -> Stack bool
+  Stack bool
   (requires fun h -> live h privKey /\ live h k /\ live h result /\ live h m /\ 
     LowStar.Monotonic.Buffer.all_disjoint [loc m; loc privKey; loc k; loc result] /\
     
@@ -312,7 +252,7 @@ val ecdsa_signature_nist_compliant: m: lbuffer uint8 (size 32) ->
 )
 
 
-let ecdsa_signature_nist_compliant m privKey k result = 
+let ecdsa_signature_nist_compliant result m privKey k = 
   push_frame();
     let h0 = ST.get() in 
     
@@ -327,7 +267,7 @@ let ecdsa_signature_nist_compliant m privKey k result =
 	    lemma_core_0 privKeyAsFelem h1;
 	    Lib.ByteSequence.uints_from_bytes_le_nat_lemma #U64 #_ #4 (as_seq h1 privKey);
 
-    let flag = ecdsa_signature_core_nist_compliant m privKeyAsFelem k r s in 
+    let flag = ecdsa_signature_core_nist_compliant r s m privKeyAsFelem k in 
       let h2 = ST.get() in 
 
       toUint8 r resultR; 
@@ -384,14 +324,14 @@ let ecdsa_signature_core mLen m privKeyAsFelem k r s =
       let tempBuffer = create (size 100) (u64 0) in 
       let kAsFelem = create (size 4) (u64 0) in 
     toUint64 k kAsFelem;  
-    ecdsa_signature_step12 mLen m hashAsFelem;
+    ecdsa_signature_step12 hashAsFelem mLen m;
 
   let h1 = ST.get() in 
       lemma_core_0 kAsFelem h1;
       uints_from_bytes_le_nat_lemma #U64 #_ #4 (as_seq h0 k);
-    let step5Flag = ecdsa_signature_step45 k tempBuffer r in 
+    let step5Flag = ecdsa_signature_step45 r k tempBuffer in 
       if not step5Flag then begin
-	ecdsa_signature_step6 kAsFelem hashAsFelem r privKeyAsFelem s;
+	ecdsa_signature_step6 s kAsFelem hashAsFelem r privKeyAsFelem;
 	pop_frame(); 
 	let step6Flag = isZero_bool s in 
 	not step6Flag
